\documentclass{article}
\usepackage{amsmath}

\begin{document}

\section{Question:}

Prove that the sum of two even integers is always even.

\section{Answer:}

Assume, for contradiction, that the sum of two even integers is odd. That is, assume:
\begin{equation}
    a + b = 2k + 1, \quad \text{for some integer } k.
\end{equation}

Since $a$ and $b$ are even, they can be written as:
\begin{equation}
    a = 2m, \quad b = 2n.
\end{equation}

Adding these values:
\begin{equation}
    a + b = 2m + 2n = 2(m+n).
\end{equation}

Since $2(m+n)$ is even, this contradicts our assumption that $a + b$ is odd. Therefore, the sum of two even numbers must be even.

\end{document}