\documentclass{article}
\usepackage{amsmath}
\usepackage{amssymb}
\title{Introduction to Addition via Recursion}
\author{}
\date{}

\begin{document}
\section{Example 2: \( 0 + 4 \)}
Using the recursive definition:
\[
    \begin{aligned}
        0 + 4 & = (0 + 3) + 1                   \\
              & = ((0 + 2) + 1) + 1             \\
              & = (((0 + 1) + 1) + 1) + 1       \\
              & = ((((0 + 0) + 1) + 1) + 1) + 1 \\
              & = (((0 + 1) + 1) + 1) + 1       \\
              & = ((1 + 1) + 1) + 1             \\
              & = (2 + 1) + 1                   \\
              & = 3 + 1                         \\
              & = 4
    \end{aligned}
\]


\end{document}

